extraction/aggregation/coq/ExtractTree.v
@@ -1,0 +1,49 @@
+Require Import Verdi.
+Require Import NPeano.
+Require Import PeanoNat.
+Require Import StructTact.Fin.
+
+Require Import NameOverlay.
+Require Import TreeStatic.
+
+Require Import ExtrOcamlBasic.
+Require Import ExtrOcamlNatInt.
+Require Import ExtrOcamlString.
+
+Extract Inlined Constant Nat.max => "Pervasives.max".
+Extract Inlined Constant Nat.min => "Pervasives.min".
+
+Extract Inlined Constant length => "List.length".
+Extract Inlined Constant negb => "not".
+Extract Inlined Constant app => "List.append".
+Extract Inlined Constant map => "List.map".
+Extract Inlined Constant rev => "List.rev".
+Extract Inlined Constant filter => "List.filter".
+Extract Inlined Constant fold_left => "(fun a b c -> List.fold_left a c b)".
+Extract Inlined Constant in_dec => "(fun h -> List.mem)".
+Extract Inlined Constant leb => "(<=)".
+Extract Inlined Constant Nat.ltb => "(<)".
+Extract Inlined Constant Nat.pred => "(fun n -> if n <= 0 then 0 else n - 1)".
+
+Extract Inlined Constant fin => int.
+
+Extract Inlined Constant fin_eq_dec => "(fun _ -> (=))".
+Extract Inlined Constant all_fin => "(fun n -> (Obj.magic (seq 1 n)))".
+
+Module N5 : NatValue. Definition n := 5. End N5.
+
+Module FN_N5 : FinNameType N5 := FinName N5.
+Module NOT_N5 : NameOrderedType FN_N5 := FinNameOrderedType N5 FN_N5.
+Module NOTC_N5 : NameOrderedTypeCompat FN_N5 := FinNameOrderedTypeCompat N5 FN_N5.
+Module ANC_N5 := FinCompleteAdjacentNameType N5 FN_N5.
+
+Require Import MSetList.
+Module N5Set <: MSetInterface.S := MSetList.Make NOT_N5.
+
+Require Import FMapList.
+Module N5Map <: FMapInterface.S := FMapList.Make NOTC_N5.
+Module RNT_N5 := FinRootNameType N5 FN_N5.
+
+Module T := Tree FN_N5 NOT_N5 N5Set NOTC_N5 N5Map RNT_N5 ANC_N5.
+
+Extraction "Tree.ml" T.Tree_BaseParams T.Tree_MultiParams.
